address a bunch of review comments

cedar-lean/Cedar/Spec/Authorizer.lean
@@ -27,13 +27,6 @@ open Effect
 def satisfied (policy : Policy) (req : Request) (entities : Entities) : Bool :=
   (evaluate policy.toExpr req entities) = .ok true
 
-/--
-  Despite its name, this function is not just a version of `satisfied` that takes
-  into account the `effect`.
-
-  While `satisfied` returns Bool, `satisfiedWithEffect` returns `Option PolicyID`
-  with the policy's id if it is satisfied.
--/
 def satisfiedWithEffect (effect : Effect) (policy : Policy) (req : Request) (entities : Entities) : Option PolicyID :=
   if policy.effect == effect && satisfied policy req entities
   then some policy.id
@@ -52,18 +45,18 @@ def hasError (policy : Policy) (req : Request) (entities : Entities) : Bool :=
   `Option PolicyID`, but not analogous to `satisfiedWithEffect` in that it does
   not consider the policy's effect.
 -/
-def idIfHasError (policy : Policy) (req : Request) (entities : Entities) : Option PolicyID :=
+def errored (policy : Policy) (req : Request) (entities : Entities) : Option PolicyID :=
   if hasError policy req entities then some policy.id else none
 
 def errorPolicies (policies : Policies) (req : Request) (entities : Entities) : Set PolicyID :=
-  Set.make (policies.filterMap (idIfHasError · req entities))
+  Set.make (policies.filterMap (errored · req entities))
 
 def isAuthorized (req : Request) (entities : Entities) (policies : Policies) : Response :=
   let forbids := satisfiedPolicies .forbid policies req entities
   let permits := satisfiedPolicies .permit policies req entities
-  let error_policies := errorPolicies policies req entities
+  let erroredPolicies := errorPolicies policies req entities
   if forbids.isEmpty && !permits.isEmpty
-  then { decision := .allow, determining_policies := permits, error_policies }
-  else { decision := .deny,  determining_policies := forbids, error_policies }
+  then { decision := .allow, determiningPolicies := permits, erroredPolicies }
+  else { decision := .deny,  determiningPolicies := forbids, erroredPolicies }
 
 end Cedar.Spec
